theories/clang/tactics.v
@@ -1,0 +1,122 @@
+Require Import clang.logic.
+From iris.proofmode Require Import coq_tactics tactics.
+Set Default Proof Using "Type".
+Import uPred.
+
+(** The tactic [reshape_expr e tac] decomposes the expression [e] into an
+evaluation context [K] and a subexpression [e']. It calls the tactic [tac K e']
+for each possible decomposition until [tac] succeeds. *)
+
+Ltac reshape_expr e tac :=
+  let rec go K e :=
+  match e with
+  | _ => tac (reverse K) e
+  | Ebinop ?op (Evalue ?v1) ?e2 => go (EKbinopl op v1 :: K) e2
+  | Ebinop ?op ?e1 ?e2 => go (EKbinopr op e2 :: K) e1
+  (* | If ?e0 ?e1 ?e2 => go (IfCtx e1 e2 :: K) e0 *)
+  (* | Pair ?e1 ?e2 => reshape_val e1 ltac:(fun v1 => go (PairRCtx v1 :: K) e2) *)
+  (* | Pair ?e1 ?e2 => go (PairLCtx e2 :: K) e1 *)
+  (* | Fst ?e => go (FstCtx :: K) e *)
+  (* | Snd ?e => go (SndCtx :: K) e *)
+  (* | InjL ?e => go (InjLCtx :: K) e *)
+  (* | InjR ?e => go (InjRCtx :: K) e *)
+  (* | Case ?e0 ?e1 ?e2 => go (CaseCtx e1 e2 :: K) e0 *)
+  (* | Alloc ?e => go (AllocCtx :: K) e *)
+  | Ederef ?e => go (EKderef :: K) e
+  (* | Store ?e1 ?e2 => reshape_val e1 ltac:(fun v1 => go (StoreRCtx v1 :: K) e2) *)
+  (* | Store ?e1 ?e2 => go (StoreLCtx e2 :: K) e1 *)
+  (* | CAS ?e0 ?e1 ?e2 => reshape_val e0 ltac:(fun v0 => first *)
+  (*    [ reshape_val e1 ltac:(fun v1 => go (CasRCtx v0 v1 :: K) e2) *)
+  (*    | go (CasMCtx v0 e2 :: K) e1 ]) *)
+  (* | CAS ?e0 ?e1 ?e2 => go (CasLCtx e1 e2 :: K) e0 *)
+  end in go (@nil exprctx) e.
+
+Ltac reshape_stmts s tac :=
+  match s with
+    | Sassign (Evalue (Vptr ?l)) ?e =>
+      reshape_expr e ltac:(fun Kes e' => tac Kes (SKassignl l) e')
+    | Srete ?e =>
+      reshape_expr e ltac:(fun Kes e' => tac Kes SKrete e')
+  end.
+
+(* Ltac reshape_cur cur tac := *)
+(*   match cur with *)
+(*     | cure ?e => reshape_expr e ltac:(fun K e' => tac K (cure e')) *)
+(*     | curs ?s => reshape_stmts s tac *)
+  (* end. *)
+
+Ltac wp_bind_e_core K :=
+  lazymatch eval hnf in K with
+  | [] => idtac
+  | _ => etrans; [|fast_by apply (wp_bind_e K)]; simpl
+  end.
+
+Tactic Notation "wp_bind_e" open_constr(efoc) :=
+  iStartProof;
+  lazymatch goal with
+  | |- _ ⊢ wp ?E (cure ?e) ?Q ?P => reshape_expr e ltac:(fun K e' =>
+    match e' with
+    | efoc => unify e' efoc; wp_bind_e_core K
+    end) || fail "wp_bind_e: cannot find" efoc "in" e
+  | _ => fail "wp_bind_e: not a 'wp'"
+  end.
+
+Ltac wp_bind_core Kes Ks :=
+  lazymatch eval hnf in Kes with
+  | [] => etrans; [|fast_by apply (wp_bind [] Ks)]; simpl
+  | _ => etrans; [|fast_by apply (wp_bind Kes Ks)]; simpl
+  end.
+
+Tactic Notation "wp_bind" open_constr(efoc) :=
+  iStartProof;
+  lazymatch goal with
+  | |- _ ⊢ wp ?E (curs ?s) ?Q ?P => reshape_stmts s ltac:(fun Kes Ks e' =>
+    match e' with
+    | efoc => unify e' efoc; wp_bind_core Kes Ks
+    end) || fail "wp_bind: cannot find" efoc "in" s
+  | _ => fail "wp_bind: not a 'wp'"
+  end.
+
+
+(* Section heap. *)
+(* Context `{clangG Σ}. *)
+
+(* Lemma tac_wp_assign Δ Δ' Δ'' E i l (v v': val) (t t': type) Φ Φret: *)
+(*   typeof t' v' → *)
+(*   IntoLaterNEnvs 1 Δ Δ' → *)
+(*   envs_lookup i Δ' = Some (false, l ↦ v @ t)%I → *)
+(*   envs_simple_replace i false (Esnoc Enil i (l ↦ v' @ t')) Δ' = Some Δ'' → *)
+(*   (Δ'' ⊢ Φ Vvoid) → *)
+(*   Δ ⊢ WP curs (Sassign (Evalue (Vptr l)) (Evalue v')) @ E {{ Φ ; Φret }}. *)
+(* Proof. *)
+(*   intros. eapply wand_apply. *)
+(*   { iIntros "HP HQ". iApply wp_assign; first done. *)
+(*     iSplitL "HP"; eauto. } *)
+(*   rewrite into_laterN_env_sound -later_sep envs_simple_replace_sound //; simpl. *)
+(*   rewrite right_id. apply later_mono, sep_mono_r, wand_mono=>//. *)
+(* Qed. *)
+
+
+(* Tactic Notation "wp_assign" := *)
+(*   iStartProof; *)
+(*   lazymatch goal with *)
+(*   | |- _ ⊢ wp ?E ?cur ?Q ?P => *)
+(*     first *)
+(*       [reshape_expr cur ltac:(fun K cur' => *)
+(*          match eval hnf in cur' with (curs (Sassign _ _)) => wp_bind_core K end) *)
+(*       |fail 1 "wp_assign: cannot find 'Sassign' in" cur]; *)
+(*     eapply tac_wp_assign; *)
+(*       [let cur' := match goal with |- to_val ?cur' = _ => cur' end in *)
+(*        auto (* wp_done *) || fail "wp_assign:" cur' "not a value" *)
+(*       |apply _ *)
+(*       |let l := match goal with |- _ = Some (_, (?l ↦{_} _ @ _)%I) => l end in *)
+(*        iAssumptionCore || fail "wp_assign: cannot find" l "↦ ? @ ?" *)
+(*       |env_cbv; reflexivity *)
+(*       | auto (* wp_finish *)] *)
+(*   | _ => fail "wp_assign: not a 'wp'" *)
+(*   end. *)
+
+
+(* End heap. *)
+
+
